fairis/heap_lang/examples/even_odd/thread_progs.v
@@ -14,22 +14,30 @@ From trillium.fairness.heap_lang.examples.even_odd Require Import action_model.
 Close Scope Z. 
 
 
-Class threadG Σ := ThreadG {
-  th_name: gname;
-  th_n_G :> inG Σ (excl_authR natO);
-}.
-
-Class threadPreG Σ := {
-  thread_PreG :> inG Σ (excl_authR natO);
-}.
-
-
 Section ThreadGLemmas.
+  Class threadG Σ := ThreadG {
+    th_name: gname;
+    th_n_G :> inG Σ (excl_authR natO);
+  }.
+
+  Class threadPreG Σ := {
+    thread_PreG :> inG Σ (excl_authR natO);
+  }.
+
+  Lemma th_alloc `{threadPreG Σ} (M: nat):
+    ⊢ |==> ∃ γ, own γ (◯E M) ∗ own γ (●E M).
+  Proof.
+    iStartProof.
+    iMod (own_alloc (●E M  ⋅ ◯E _))%nat as (γ) "[AUTH FRAG]".
+    { apply auth_both_valid_2; eauto. by compute. }
+    by iFrame.
+  Qed. 
+  
   Context `{!threadG Σ}.
 
   Definition th_at (n: nat) := own th_name (◯E n).
   Definition auth_th_at (n: nat) := own th_name (●E n).
-  
+
   Lemma th_agree γ (N M: nat) :
     own γ (◯E N) -∗ own γ (●E M) -∗ ⌜ M = N ⌝.
   Proof.
@@ -47,19 +55,89 @@ Section ThreadGLemmas.
 End ThreadGLemmas.
 
 
-(* exposing the new fuel amount, since lm_fl depends on the new M state which is not available *)
+Record StateRes {Σ: gFunctors} (cond: nat -> bool) (sr_auth sr_frag: nat -> iProp Σ) := {    
+    sr_agree: ∀ n m, sr_frag n -∗ sr_auth m -∗ 
+                      ⌜ n = (if cond m then m else m + 1)%nat ⌝;
+    sr_upd: ∀ n, sr_frag n -∗ sr_auth n ==∗
+                   sr_frag (if cond n then n + 2 else n) ∗
+                   sr_auth (if cond n then n + 1 else n);
+}.
+
+
+Section StResImpl.
+  Context `{!threadPreG Σ}.
+
+  Section Impl.
+    Context (even_name odd_name: gname).
+    
+    Local Instance evenThreadG: threadG Σ := {| th_name := even_name |}. 
+    Local Instance oddThreadG: threadG Σ := {| th_name := odd_name |}. 
+    
+    Local Definition even_at := (@th_at _ evenThreadG). 
+    Local Definition odd_at := (@th_at _ oddThreadG). 
+    
+    Local Definition auth_even_at := (@auth_th_at _ evenThreadG). 
+    Local Definition auth_odd_at := (@auth_th_at _ oddThreadG).  
+    
+    Local Definition st_res N: iProp Σ :=
+      if Nat.even N
+      then (auth_even_at N ∗ auth_odd_at (N+1))%I
+      else (auth_even_at (N+1) ∗ auth_odd_at N)%I.
+    
+    Lemma st_res_SR_even: @StateRes _ Nat.even st_res even_at.
+      split.
+      - rewrite /st_res. setoid_rewrite if_arg2_comm. iIntros (??) "TH [EVEN ODD]".
+        rewrite !if_arg_comm.
+        by iDestruct (th_agree with "[$] [$]") as %->.
+      - rewrite /st_res. setoid_rewrite if_arg2_comm. iIntros (?) "TH [EVEN ODD]".
+        rewrite !if_arg_comm.
+        destruct (Nat.even n) eqn:E.
+        2: { rewrite E. by iFrame. }
+        rewrite even_plus1_negb E -Nat.add_assoc. simpl.
+        iMod (th_update with "[EVEN TH]") as "[??]"; by iFrame.
+    Qed.
+    
+    Lemma st_res_SR_odd: @StateRes _ Nat.odd st_res odd_at.
+    Proof.
+      split.
+      - rewrite /st_res. setoid_rewrite if_arg2_comm. iIntros (??) "TH [EVEN ODD]".
+        rewrite !if_arg_comm.
+        rewrite -(negb_if _ _ _ (Nat.odd m)) Nat.negb_odd.
+        by iDestruct (th_agree with "[$] [$]") as %->.
+      - rewrite /st_res. setoid_rewrite if_arg2_comm. iIntros (?) "TH [EVEN ODD]".
+        rewrite if_arg_comm.
+        rewrite -!(negb_if _ _ _ (Nat.odd n)) Nat.negb_odd.
+        destruct (Nat.even n) eqn:E.
+        { rewrite E. by iFrame. }
+        rewrite even_plus1_negb E -Nat.add_assoc. simpl.
+        iMod (th_update with "[ODD TH]") as "[??]"; by iFrame.
+    Qed.
+
+  End Impl.
+
+  (* we only use it for even n, but generalization for arbitrary n is possible *)
+  Lemma st_res_init n (EVEN: Nat.even n):
+    ⊢ |==> ∃ st_res even_at odd_at,
+        st_res n ∗ even_at n ∗ odd_at (n + 1) ∗
+          ⌜ @StateRes Σ Nat.even st_res even_at ⌝ ∗
+          ⌜ @StateRes Σ Nat.odd st_res odd_at ⌝.
+  Proof using threadPreG0.
+    iMod (th_alloc n) as (γ1) "[AUTH1 FRAG1]". 
+    iMod (th_alloc (n + 1)) as (γ2) "[AUTH2 FRAG2]".
+    iModIntro. do 3 iExists _. rewrite !bi.sep_assoc.
+    iSplitL.
+    2: { iPureIntro. apply (st_res_SR_odd γ1 γ2). }
+    iSplitL.
+    2: { iPureIntro. apply (st_res_SR_even γ1 γ2). }
+    apply Is_true_true_1 in EVEN. rewrite /st_res EVEN. iFrame. 
+  Qed. 
+
+End StResImpl. 
+
+
 Definition MU__r `{LM: LiveModel heap_lang M} `{!heapGS Σ LM} ρ E τ P: iProp Σ :=  
   ∀ f R, τ ↦M ({[ ρ := f ]} ∪ (S <$> R)) ∗ ⌜ ρ ∉ dom R ⌝ -∗
           MU E τ (τ ↦M ({[ ρ := lm_flm LM ]} ∪ R) ∗ P).
-
-
-Record StateRes `{!threadG Σ} (cond: nat -> bool) (sr: nat -> iProp Σ) := {    
-    sr_th_agree: ∀ n m, th_at n -∗ sr m -∗ 
-                         ⌜ n = (if cond m then m else m + 1)%nat ⌝;
-    sr_th_upd: ∀ n, th_at n -∗ sr n ==∗
-                                 th_at (if cond n then n + 2 else n) ∗
-                                 sr (if cond n then n + 1 else n);
-}.
 
 
 Section ProofsGen.  
@@ -67,21 +145,19 @@ Section ProofsGen.
   Context `{!heapGS Σ LM__p}.
   Context (cond: nat -> bool).
   Hypothesis (COND_S_NEG: forall n, cond (S n) = negb (cond n)). 
-  
-  Context `{!threadG Σ}.
-  
+    
   Definition incr_loop : val :=
     rec: "incr_loop" "l" "n" :=
       (if: CAS "l" "n" ("n"+ #1)
        then "incr_loop" "l" ("n" + #2)
        else "incr_loop" "l" "n").
 
-  Definition eo_corr `(SR: StateRes cond sr) l (N: nat): iProp Σ :=
+  Definition eo_corr `(SR: StateRes cond sr frag) l (N: nat): iProp Σ :=
     l ↦ #N ∗
     sr N.
     (* own th_name (●E (if cond N then N else (N + 1))). *)
   
-  Definition eo_vs `(SR: StateRes cond sr) l ι (ρ: fmrole M__p) tid : iProp Σ :=
+  Definition eo_vs `(SR: StateRes cond sr frag) l ι (ρ: fmrole M__p) tid : iProp Σ :=
     □ |={⊤, ⊤ ∖ ↑ι}=> ∃ N,
       (▷ eo_corr SR l N) ∗
       (MU__r ρ (⊤ ∖ ↑ι) tid
@@ -89,15 +165,15 @@ Section ProofsGen.
       ).
 
   Definition eo_spec (prog: val) :=
-    forall `(SR: StateRes cond sr) (tid: locale heap_lang) n ρ (N: nat) f (Hf: f > 40) ι
+    forall `(SR: StateRes cond sr frag) (tid: locale heap_lang) n ρ (N: nat) f (Hf: f > 40) ι
     (FL: lm_flm LM__p >= 61),
-    ⊢ {{{ eo_vs SR n ι ρ tid ∗ has_fuels tid {[ ρ := f ]} ∗ own th_name (◯E N) }}}
+    ⊢ {{{ eo_vs SR n ι ρ tid ∗ has_fuels tid {[ ρ := f ]} ∗ frag N }}}
         prog #n #N @ tid
       {{{ RET #(); has_fuels tid ∅ }}}.    
   
   Lemma eo_spec_incr_loop: eo_spec incr_loop.
   Proof using COND_S_NEG.
-    red. intros sr SR tid n ρ N f Hf ι FL.
+    red. intros sr frag SR tid n ρ N f Hf ι FL.
     iIntros "!>". 
     iLöb as "Hg" forall (N f Hf).
     iIntros (Φ). iIntros "(#VS & Hf & Heven) Hk".
@@ -116,8 +192,7 @@ Section ProofsGen.
     rewrite map_union_empty.
 
     iAssert (▷ ⌜ _ ⌝)%I with "[Heven SR]" as "#EQ".
-    { iNext.
-      iApply (sr_th_agree _ _ SR with "[$] [$]"). }
+    { iNext. iApply (sr_agree _ _ _ SR with "[$] [$]"). }
     iMod "EQ" as "%".
             
     destruct (cond M) eqn:Heqn.
@@ -128,7 +203,7 @@ Section ProofsGen.
       iApply (MU_wand with "[-CLOS] [$]"). 
       iIntros "(Hf & CLOS)". 
 
-      iMod (sr_th_upd _ _ SR with "[$] [$]") as "[Heven Hay]". rewrite Heqn. 
+      iMod (sr_upd _ _ _ SR with "[$] [$]") as "[Heven Hay]". rewrite Heqn. 
       wp_pures.
       iModIntro. 
       iMod ("CLOS" with "[Hay Hb]") as "_". 
@@ -169,13 +244,13 @@ End ProofsGen.
 
 Record EvenProg := {
     e_prog: val;
-    e_spec `{LM__p: LiveModel heap_lang M__p} `{!heapGS Σ LM__p, !threadG Σ}:
+    e_spec `{LM__p: LiveModel heap_lang M__p} `{!heapGS Σ LM__p}:
       eo_spec Nat.even e_prog;
 }.
 
 Record OddProg := {
     o_prog: val;
-    o_spec `{LM__p: LiveModel heap_lang M__p} `{!heapGS Σ LM__p, !threadG Σ}:
+    o_spec `{LM__p: LiveModel heap_lang M__p} `{!heapGS Σ LM__p}:
       eo_spec Nat.odd o_prog;
 }.
 
